coq: set theory

coq/Logic/Lang1/Context.v
@@ -56,56 +56,21 @@ Proof.
     intros G n m x y H1 H2. constructor; assumption.
 Qed.
 
-(* Just so the predicate Eval can have two arguments instead of three.          *)
-Inductive Interpretation : Type :=
-| mkInterp : forall (p:Formula) (A:Prop), Interpretation
-.
+Definition inclCtx (G H:Context) : Prop :=
+    forall (n:nat) (x:set), G :> n~>x -> H :> n~>x.
 
-Notation "p ~ P" := (mkInterp p P)
-    (at level 1, no associativity) : Context_scope.
+Notation "G <= H"  := (inclCtx G H)
+    (at level 70, no associativity) : Context_scope.
 
 Open Scope Context_scope.
 
-Inductive Eval : Context -> Interpretation -> Prop :=
-| EvalBot  : forall (G:Context), Eval G Bot ~ False
-| EvalElem : forall (G:Context) (n m:nat) (x y:set),
-    G :> n~>x -> G :> m~>y -> Eval G (Elem n m) ~ (x :: y)
-| EvalImp  : forall (G:Context) (p1 p2:Formula) (A1 A2:Prop), 
-    Eval G p1 ~ A1 -> Eval G p2 ~ A2 -> Eval G (Imp p1 p2) ~ (A1 -> A2)
-|EvalAll   : forall (G:Context) (n:nat) (p1:Formula) (A1:set -> Prop),
-    (forall (x:set), Eval (G ; n~>x) p1 ~ (A1 x)) ->
-    Eval G (All n p1) ~ (forall (x:set), A1 x)
-.
-
-Notation "G :- I" := (Eval G I)
-    (at level 60, no associativity).
-
-Open Scope Context_scope.
-
-(* Just restating constructor EvalBot with custom notations.                    *)
-Lemma evalBot : forall (G:Context), G :- Bot ~ False.
+(*
+Lemma inclCtxExtend : forall (G H:Context) (n:nat) (x:set),
+    G <= H -> G ; n~>x <= H ; n~>x.
 Proof.
-    intros G. constructor.
-Qed.
-
-(* Just restating constructor EvalElem with custom notations.                   *)
-Lemma evalElem : forall (G:Context) (n m:nat) (x y:set),
-    G :> n~>x -> G :> m~>y -> G :- (Elem n m) ~ (x :: y).
-Proof.
-    intros G n m x y H1 H2. constructor; assumption.
-Qed.
-
-(* Just restating constructor EvalImp with custom notations.                    *)
-Lemma evalImp : forall (G:Context) (p1 p2:Formula) (A1 A2:Prop),
-    G :- p1 ~ A1 -> G :- p2 ~ A2 -> G :- (Imp p1 p2) ~ (A1 -> A2).
-Proof.
-    intros G p1 p2 A1 A2 H1 H2. constructor; assumption.
-Qed.
-
-(* Just restating constructor EvalAll with custom notations.                    *)
-Lemma evalAll : forall (G:Context) (n:nat) (p1:Formula) (A1:set -> Prop),
-    (forall (x:set), G ; n~>x :- p1 ~ (A1 x)) -> 
-        G :- (All n p1) ~ (forall (x:set), A1 x).
-Proof.
-    intros G n p1 A1 H1. constructor. assumption.
-Qed.
+    intros G H n x. unfold inclCtx. intros H2 m y H3.
+    remember (G ; n~>x) as G' eqn:G1. remember (H ; n~>x) as H' eqn:H1. 
+    revert G1 H1.
+    
+Show.
+*)
